@prefix owl: <http://www.w3.org/2002/07/owl#> .
@prefix dc:  <http://purl.org/dc/terms/> .
@prefix prov: <http://www.w3.org/ns/prov#> .
@prefix time: <http://www.w3.org/2006/time#> .
@prefix rdf: <http://www.w3.org/1999/02/22-rdf-syntax-ns#> .
@prefix rdfs: <http://www.w3.org/2000/01/rdf-schema#> .
@prefix xsd: <http://www.w3.org/2001/XMLSchema#> .
@prefix upper: <https://w3id.org/schweidler/semantics/qa-kg/upper#> .
@prefix mer: <https://w3id.org/schweidler/semantics/qa-kg/meronymy#> .
@prefix gloss: <https://w3id.org/schweidler/semantics/qa-kg/glossary#> .
@prefix : <https://w3id.org/schweidler/semantics/qa-kg#> .

#################################################################
# Documentation
#################################################################
<https://w3id.org/schweidler/semantics/qa-kg/qa>
    a owl:Ontology ;
    dc:title "Software Quality Assurance Domain Ontology" ;
    dc:creator "Ren√© Schweidler MSc." ;
    dc:description "Ontology modeling entities that belong to the domain of software quality assurance and testing however are independent from scrum."@en ;
    rdfs:label "Software Quality Assurance Domain Ontology" ;
    owl:versionInfo "0.1" ;
    owl:imports
        <http://www.w3.org/ns/prov#> ,
        <http://www.w3.org/2006/time#> ,
        <http://www.w3.org/2002/07/owl#> ,
        <http://purl.org/dc/terms/> ,
        <http://www.w3.org/1999/02/22-rdf-syntax-ns#> ,
        <http://www.w3.org/2000/01/rdf-schema#> ,
        <http://www.w3.org/2001/XMLSchema#> ,
        <https://w3id.org/schweidler/semantics/qa-kg/upper#> ,
        <https://w3id.org/schweidler/semantics/qa-kg/meronymy#> ,
        <https://w3id.org/schweidler/semantics/qa-kg/glossary#> ,
        <https://w3id.org/schweidler/semantics/qa-kg#> .

#################################################################
# Core Classes
#################################################################
:SoftwareFunction a owl:Class ;
    rdfs:label "Software Function"@en ;
    rdfs:comment "A distinct capability or behavior implemented by software to fulfill one or more requirements."@en ;
    skos:scopeNote "Use this concept to represent an individual, identifiable piece of software behavior or functionality, typically aligned with a requirement or user need. It is not intended to represent entire systems, subsystems, or non-functional aspects like performance or scalability."@en ;
    skos:exactMatch gloss:SoftwareFunctionConcept ;
    rdfs:isDefinedBy gloss:SoftwareFunctionConcept ;
    rdfs:subClassOf upper:Artifact .

:Requirement a owl:Class ;
    rdfs:label "Requirement"@en ;
    rdfs:comment "A documented condition or capability needed by a stakeholder or system to solve a problem or achieve an objective, which must be fulfilled by a software or system component."@en ;
    skos:scopeNote "Use this concept to describe stakeholder expectations or system obligations that must be satisfied. It includes both functional and non-functional requirements, but should not be confused with implementation details or technical tasks."@en ;
    skos:exactMatch gloss:RequirementConcept ;
    rdfs:isDefinedBy gloss:RequirementConcept ;
    rdfs:subClassOf prov:Entity .

:Constraint a owl:Class ;
    rdfs:label "Constraint"@en ;
    rdfs:comment "A type of requirement that imposes a restriction on the design, implementation, or operation of a system."@en ;
    skos:scopeNote "Use this concept to classify requirements that limit how a system must be built or operated. Examples include regulatory requirements, technology constraints, interoperability obligations, or resource limitations."@en ;
    skos:exactMatch gloss:ConstraintConcept ;
    rdfs:isDefinedBy gloss:ConstraintConcept ;
    rdfs:subClassOf :Requirement .

#################################################################
# ObjectProperties
#################################################################

#################################################################
# DatatypeProperties
#################################################################

#################################################################
# Inverse ObjectProperties
#################################################################
