@prefix owl: <http://www.w3.org/2002/07/owl#> .
@prefix dct: <http://purl.org/dc/terms/> .
@prefix rdf: <http://www.w3.org/1999/02/22-rdf-syntax-ns#> .
@prefix rdfs: <http://www.w3.org/2000/01/rdf-schema#> .
@prefix skos: <http://www.w3.org/2004/02/skos/core#> .
@prefix rsont: <https://w3id.org/schweidler/semantics/qa-kg/data/ReneSchweidler#> .
@prefix xsd: <http://www.w3.org/2001/XMLSchema#> .
@prefix time: <http://www.w3.org/2006/time#> .
@prefix prov: <http://www.w3.org/ns/prov#> .
@prefix vann: <http://purl.org/vocab/vann/> .
@prefix coglo: <https://w3id.org/schweidler/semantics/qa-kg/core-glossary#> .
@prefix mevoc: <https://w3id.org/schweidler/semantics/qa-kg/meronymy-vocabulary#> .
@prefix upper: <https://w3id.org/schweidler/semantics/qa-kg/upper#> .
@prefix qavoc: <https://w3id.org/schweidler/semantics/qa-kg/qa-vocabulary#> .
@prefix qa: <https://w3id.org/schweidler/semantics/qa-kg#> .

#################################################################
# Documentation
#################################################################
<https://w3id.org/schweidler/semantics/qa-kg/qa-vocabulary>
    a owl:Ontology ;
    dct:title "Software Quality Assurance Domain Ontology" ;
    rdfs:label "Software Quality Assurance Domain Ontology" ;
    rdfs:comment "Software Quality Assurance Domain Ontology"@en ;
    dct:description "Ontology modeling entities that belong to the domain of software quality assurance and testing however are independent from scrum."@en ;
    dct:language "en" ;
    dct:creator rsont:ReneSchweidler ;
    dct:created "2025-07-05"^^xsd:date ;
    dct:modified "2025-07-02"^^xsd:date ;    
    dct:license <http://creativecommons.org/licenses/by/4.0/> ;
    vann:preferredNamespacePrefix "qavoc" ;
    vann:preferredNamespaceUri "https://w3id.org/schweidler/semantics/qa-kg/qa-vocabulary#" ;
    owl:versionIRI <https://w3id.org/schweidler/semantics/qa-kg/qa-vocabulary/0.1.0/> ;
    owl:versionInfo "0.1.0" ;
    owl:imports owl:, dct:, rdf:, rdfs:, skos:, rsont:, xsd:, owl:, time:, prov:, coglo:, mevoc:, upper:, qa:, vann: .

#################################################################
# Core Classes
#################################################################
qavoc:SoftwareFunction a owl:Class ;
    rdfs:label "Software Function"@en ;
    rdfs:comment "A distinct capability or behavior implemented by software to fulfill one or more requirements."@en ;
    skos:scopeNote "Use this concept to represent an individual, identifiable piece of software behavior or functionality, typically aligned with a requirement or user need. It is not intended to represent entire systems, subsystems, or non-functional aspects like performance or scalability."@en ;
    skos:exactMatch coglo:SoftwareFunctionConcept ;
    rdfs:isDefinedBy coglo:SoftwareFunctionConcept ;
    rdfs:subClassOf upper:Artifact .

qavoc:Requirement a owl:Class ;
    rdfs:label "Requirement"@en ;
    rdfs:comment "A documented condition or capability needed by a stakeholder or system to solve a problem or achieve an objective, which must be fulfilled by a software or system component."@en ;
    skos:scopeNote "Use this concept to describe stakeholder expectations or system obligations that must be satisfied. It includes both functional and non-functional requirements, but should not be confused with implementation details or technical tasks."@en ;
    skos:exactMatch coglo:RequirementConcept ;
    rdfs:isDefinedBy coglo:RequirementConcept ;
    rdfs:subClassOf prov:Entity .

qavoc:Constraint a owl:Class ;
    rdfs:label "Constraint"@en ;
    rdfs:comment "A type of requirement that imposes a restriction on the design, implementation, or operation of a system."@en ;
    skos:scopeNote "Use this concept to classify requirements that limit how a system must be built or operated. Examples include regulatory requirements, technology constraints, interoperability obligations, or resource limitations."@en ;
    skos:exactMatch coglo:ConstraintConcept ;
    rdfs:isDefinedBy coglo:ConstraintConcept ;
    rdfs:subClassOf qavoc:Requirement .

#################################################################
# ObjectProperties
#################################################################

#################################################################
# DatatypeProperties
#################################################################

#################################################################
# Inverse ObjectProperties
#################################################################
